Add is_valid_params

ConsensusSafety.thy
@@ -1,125 +1,8 @@
 theory ConsensusSafety
 
-imports Main
+imports Main CBCCasper
 
 begin
-
-(* Section 2: Description of CBC Casper *)
-(* Section 2.1: CBC Casper "Parameters" *)
-
-(* Definition 2.1 *)
-datatype validator = Validator int
-
-(* Definition 2.2 *)
-type_synonym weight = "validator \<Rightarrow> int"
-
-(* Definition 2.3 *)
-type_synonym threshold = int
-
-(* Definition 2.4 *)
-datatype consensus_value = Consensus_value int
-
-(* NOTE: list is used here because set can not be used for recursive definition. *)
-datatype message =
-  Message "consensus_value * validator * message list"
-
-type_synonym state = "message set"
-
-(* Definition 2.5 *)
-type_synonym estimator = "state \<Rightarrow> consensus_value set"
-
-(* NOTE: Estimator parameterized by weight. *)
-type_synonym estimator_param = "weight \<Rightarrow> estimator"
-
-(* CBC Casper parameters *)
-datatype params = 
-  Params "validator set * weight * threshold * consensus_value set * estimator_param"
-
-fun V :: "params \<Rightarrow> validator set"
-  where
-    "V (Params (v_set, _, _, _, _)) = v_set"
-
-fun W :: "params \<Rightarrow> weight"
-  where
-    "W (Params (_, weight, _, _, _)) = weight"
-
-fun t :: "params \<Rightarrow> threshold"
-  where
-    "t (Params (_, _, threshold, _, _)) = threshold"
-
-fun C :: "params \<Rightarrow> consensus_value set"
-  where
-    "C (Params (_, _, _, c_set, _)) = c_set"
-
-(* NOTE: Enforce estimator to return valid consensus values *)
-fun \<epsilon> :: "params \<Rightarrow> estimator"
-  where
-    "\<epsilon> (Params (_, weight, _, c_set, estimator_param)) = (\<lambda> \<sigma>. estimator_param weight \<sigma>  \<inter> c_set)"
-
-
-(* Section 2.2: Protocol Definition *)
-
-(* Definition 2.6 *)
-fun sender :: "message \<Rightarrow> validator"
-  where
-    "sender (Message (_, v, _)) = v"
-
-fun est :: "message \<Rightarrow> consensus_value"
-  where
-     "est (Message (c, _, _)) = c"
-
-fun justification :: "message \<Rightarrow> state"
-  where
-    "justification (Message (_, _, s)) = set s"
-
-(* Definition 2.7 *)
-definition is_valid_message :: "params \<Rightarrow> message \<Rightarrow> bool"
-  where
-    "is_valid_message params m = (est m \<in> \<epsilon> params (justification m))"
-
-fun M :: "params \<Rightarrow> message set"
-  where
-    "M params = {m. is_valid_message params m}"
-
-definition is_valid_state :: "params \<Rightarrow> state \<Rightarrow> bool"
-  where
-    "is_valid_state params \<sigma> = (\<forall> m \<in> \<sigma>. is_valid_message params m)"
-
-fun \<Sigma> :: "params \<Rightarrow> state set"
-  where
-    "\<Sigma> params = {\<sigma>. is_valid_state params \<sigma>}"
-
-(* Definition 2.8: Protocol state transitions \<rightarrow> *)
-fun is_future_state :: "(state * state) \<Rightarrow> bool"
-  where
-    "is_future_state (\<sigma>1, \<sigma>2) = (\<sigma>1 \<supseteq> \<sigma>2)"
-
-(* Definition 2.9 *)
-fun equivocation :: "(message * message) \<Rightarrow> bool"
-  where
-    "equivocation (m1, m2) =
-      (sender m1 = sender m2 \<and> m1 \<noteq> m2 \<and> m1 \<notin> justification m2 \<and> m2 \<notin> justification m1)"
-
-(* Definition 2.10 *)
-definition equivocating_validators :: "state \<Rightarrow> validator set"
-  where
-    "equivocating_validators \<sigma> = 
-      {v. \<exists> m1 m2. m1 \<in> \<sigma> \<and> m2 \<in> \<sigma> \<and> equivocation (m1, m2) \<and> sender m1 = v}"
-
-(* Definition 2.11 *)
-definition equivocation_fault_weight :: "params \<Rightarrow> state \<Rightarrow> int"
-  where
-    "equivocation_fault_weight params \<sigma> = sum (W params) (equivocating_validators \<sigma>)"
-
-(* Definition 2.12 *)
-definition is_faults_lt_threshold :: "params \<Rightarrow> state \<Rightarrow> bool"
-  where 
-    "is_faults_lt_threshold params \<sigma> = (equivocation_fault_weight params \<sigma> < t params)"
-
-fun \<Sigma>t :: "params \<Rightarrow> state set"
-  where
-    "\<Sigma>t params = {\<sigma>. is_valid_state params \<sigma> \<and> is_faults_lt_threshold params \<sigma>}"
-
 
 (* Section 3: Safety Proof *)
 (* Section 3.1: Guaranteeing Common Futures *)
@@ -131,22 +14,20 @@ fun futures :: "params \<Rightarrow> state \<Rightarrow> state set"
 
 (* Lemma 1 *)
 lemma monotonic_futures :
-  "\<forall> params \<sigma>' \<sigma>. \<sigma>' \<in> \<Sigma>t params \<and> \<sigma> \<in> \<Sigma>t params
+  "\<forall> params \<sigma>' \<sigma>. is_valid_params params \<and> \<sigma>' \<in> \<Sigma>t params \<and> \<sigma> \<in> \<Sigma>t params
    \<longrightarrow> \<sigma>' \<in> futures params \<sigma> \<longleftrightarrow> futures params \<sigma>' \<subseteq> futures params \<sigma>"
   by fastforce
 
-notation Set.empty ("\<emptyset>")
-
 (* Theorem 1 *)
 theorem two_party_common_futures :
-  "\<forall> params \<sigma>1 \<sigma>2. \<sigma>1 \<in> \<Sigma>t params \<and> \<sigma>2 \<in> \<Sigma>t params
+  "\<forall> params \<sigma>1 \<sigma>2. is_valid_params params \<and> \<sigma>1 \<in> \<Sigma>t params \<and> \<sigma>2 \<in> \<Sigma>t params
   \<longrightarrow> (\<sigma>1 \<union> \<sigma>2) \<in> \<Sigma>t params
   \<longrightarrow> futures params \<sigma>1 \<inter> futures params \<sigma>2 \<noteq> \<emptyset>"
   by auto
 
 (* Theorem 2 *)
 theorem n_party_common_futures :
-  "\<forall> params \<sigma>_set. \<sigma>_set \<subseteq> \<Sigma>t params
+  "\<forall> params \<sigma>_set. is_valid_params params \<and> \<sigma>_set \<subseteq> \<Sigma>t params
   \<longrightarrow> \<Union> \<sigma>_set \<in> \<Sigma>t params
   \<longrightarrow> \<Inter> {futures params \<sigma> | \<sigma>. \<sigma> \<in> \<sigma>_set} \<noteq> \<emptyset>"
   by auto
@@ -168,7 +49,7 @@ fun state_property_is_decided :: "params \<Rightarrow> (state_property * state) 
 
 (* Lemma 2 *)
 lemma forward_consistency :
-  "\<forall> params \<sigma>' \<sigma>. \<sigma>' \<in> \<Sigma>t params \<and> \<sigma> \<in> \<Sigma>t params
+  "\<forall> params \<sigma>' \<sigma>. is_valid_params params \<and> \<sigma>' \<in> \<Sigma>t params \<and> \<sigma> \<in> \<Sigma>t params
   \<longrightarrow> \<sigma>' \<in> futures params \<sigma> 
   \<longrightarrow> state_property_is_decided params (p, \<sigma>)
   \<longrightarrow> state_property_is_decided params (p, \<sigma>')"
@@ -177,7 +58,7 @@ lemma forward_consistency :
 
 (* Lemma 3 *)
 lemma backword_consistency :
-  "\<forall> params \<sigma>' \<sigma>. \<sigma>' \<in> \<Sigma>t params \<and> \<sigma> \<in> \<Sigma>t params
+  "\<forall> params \<sigma>' \<sigma>. is_valid_params params \<and> \<sigma>' \<in> \<Sigma>t params \<and> \<sigma> \<in> \<Sigma>t params
   \<longrightarrow> \<sigma>' \<in> futures params \<sigma> 
   \<longrightarrow> state_property_is_decided params (p, \<sigma>')
   \<longrightarrow> \<not>state_property_is_decided params (state_property_not p, \<sigma>)"
@@ -186,7 +67,7 @@ lemma backword_consistency :
   
 (* Theorem 3 *)
 theorem two_party_consensus_safety :
-  "\<forall> params \<sigma>1 \<sigma>2. \<sigma>1 \<in> \<Sigma>t params \<and> \<sigma>2 \<in> \<Sigma>t params
+  "\<forall> params \<sigma>1 \<sigma>2. is_valid_params params \<and> \<sigma>1 \<in> \<Sigma>t params \<and> \<sigma>2 \<in> \<Sigma>t params
   \<longrightarrow> (\<sigma>1 \<union> \<sigma>2) \<in> \<Sigma>t params
   \<longrightarrow> \<not>(state_property_is_decided params (p, \<sigma>1) \<and> state_property_is_decided params (state_property_not p, \<sigma>2))"
   by auto
@@ -208,7 +89,7 @@ fun state_property_decisions :: "params \<Rightarrow> state \<Rightarrow> state_
 
 (* Theorem 4 *)
 theorem n_party_safety_for_state_properties :
-  "\<forall> params \<sigma>_set. \<sigma>_set \<subseteq> \<Sigma>t params
+  "\<forall> params \<sigma>_set. is_valid_params params \<and> \<sigma>_set \<subseteq> \<Sigma>t params
   \<longrightarrow> \<Union> \<sigma>_set \<in> \<Sigma>t params
   \<longrightarrow> state_properties_are_consistent params (\<Union> {state_property_decisions params \<sigma> | \<sigma>. \<sigma> \<in> \<sigma>_set})" 
   by auto 
@@ -228,12 +109,9 @@ fun consensus_value_properties_are_consistent :: "params \<Rightarrow> consensus
     "consensus_value_properties_are_consistent params q_set = (\<exists> c \<in> C params. \<forall> q \<in> q_set. q c)"
 
 
-lemma estimates_are_valid:
-  "\<forall> params c. c \<in> \<epsilon> params \<sigma> \<longrightarrow> c \<in> C params"
-  by (metis C.simps IntE \<epsilon>.elims)  
-
 lemma extend_state_properties_are_consistent_def :
-  "\<forall> params q_set. state_properties_are_consistent params {naturally_corresponding_state_property params q | q. q \<in> q_set}
+  "\<forall> params q_set. is_valid_params params
+    \<longrightarrow> state_properties_are_consistent params {naturally_corresponding_state_property params q | q. q \<in> q_set}
     \<longrightarrow> (\<exists> \<sigma> \<in> \<Sigma> params. \<forall> p \<in> {\<lambda>\<sigma>'. \<forall> c \<in> \<epsilon> params \<sigma>'. q c | q. q \<in> q_set}. p \<sigma>)"
   apply simp
   done
